moving some code around, improved compositional memory symbolic evaluator.

examples/AutoSep.v
@@ -3,70 +3,36 @@ Export Bedrock.
 
 (** * Specialize the library proof automation to some parameters useful for basic examples. *)
 
-Import SymIL.BedrockEvaluator.
+Import SymIL.
 Require Bedrock.sep.PtsTo2.
 
 (** Build our memory plugin **)
-Module Plugin_PtsTo := Bedrock.sep.PtsTo2.BedrockPtsToEvaluator SymIL.PLUGIN.
-
-Definition master_plugin types' :=
-  let types := Env.repr SymIL.bedrock_types_r types' in
-  @PluginEvaluator.Plugin_SymEvaluator types (Expr.tvType 0) (Expr.tvType 1)
-  ((0, Plugin_PtsTo.MemEval_ptsto32 _) :: nil).
-
-Definition master_plugin_correct types' (_ _ : Expr.tvar) funcs sfuncs : 
-  (forall F, F sfuncs -> F (Plugin_PtsTo.ptsto32_ssig _ :: tl sfuncs)) ->
-  SymEvaluator_correct funcs sfuncs (master_plugin types').
-Proof.
-  simpl in *. intros.
-  generalize PluginEvaluator.Plugin_SymEvaluator_correct.
-  unfold master_plugin, PluginEvaluator.pcT, PluginEvaluator.stT.
-Admitted.
-
-Ltac prover_unfolder H :=
-  match H with
-    | tt => 
-      cbv delta [
-        EquivDec_nat
-        Provers.transitivityProver
-        Provers.transitivity_summary Provers.transitivitySummarize Provers.transitivityLearn Provers.transitivityProve
-        Provers.transitivityEqProver
-        Provers.in_seq Provers.inSameGroup Provers.eqD_seq
-        Provers.groupsOf Provers.groupWith Provers.addEquality
-      ]
-    | _ => 
-      cbv delta [
-        EquivDec_nat
-        Provers.transitivityProver
-        Provers.transitivity_summary Provers.transitivitySummarize Provers.transitivityLearn Provers.transitivityProve
-        Provers.transitivityEqProver
-        Provers.in_seq Provers.inSameGroup Provers.eqD_seq
-        Provers.groupsOf Provers.groupWith Provers.addEquality
-      ] in H
-  end.
+Module Plugin_PtsTo := Bedrock.sep.PtsTo2.BedrockPtsToEvaluator.
 
 Ltac sym_eval_simplifier H :=
-  prover_unfolder H ;
-  cbv delta [
-    master_plugin PluginEvaluator.Plugin_SymEvaluator
-    Plugin_PtsTo.MemEval_ptsto32
-    Plugin_PtsTo.sym_read_word_ptsto32
-    Plugin_PtsTo.sym_write_word_ptsto32
-    Plugin_PtsTo.expr_equal
-    SymIL.BedrockEvaluator.DefaultEvaluator.defaultLearnHook
-  ] in H;
-  PluginEvaluator.unfolder H.
+  Provers.unfold_transitivityProver H ;
+  SymIL.MEVAL.Plugin.unfolder H ;
+  cbv delta [ 
+    Plugin_PtsTo.MemEval_ptsto32 Plugin_PtsTo.ptsto32_ssig 
+    IL_mem_satisfies IL_ReadWord IL_WriteWord
+    MEVAL.Plugin.smem_read MEVAL.Plugin.smem_write
 
+    Plugin_PtsTo.expr_equal
+    Plugin_PtsTo.sym_read_word_ptsto32 Plugin_PtsTo.sym_write_word_ptsto32
+
+    Demo.defaultLearnHook
+
+    Plugin_PtsTo.ptsto32_types_r
+  ] in H ;
+  sym_evaluator H.
+  
 Ltac the_cancel_simplifier :=
-  prover_unfolder tt ;
+  Provers.unfold_transitivityProver tt ;
   cbv beta iota zeta delta 
-    [ SepTac.SEP.CancelSep projT1
-      SepTac.SEP.hash SepTac.SEP.hash' SepTac.SEP.sepCancel
+    [ ILTac.SEP.CancelSep projT1
+      ILTac.SEP.hash ILTac.SEP.hash' ILTac.SEP.sepCancel
 
       SepExpr.FM.fold
-
-      Provers.Learn Provers.Summarize Provers.Prove 
-      Provers.transitivityProver
 
       ExprUnify.Subst
 
@@ -75,23 +41,23 @@ Ltac the_cancel_simplifier :=
 
       fst snd
 
-      SepExpr.impures SepTac.SEP.star_SHeap SepExpr.FM.empty SepTac.SEP.liftSHeap
-      SepTac.SEP.sheapSubstU ExprUnify.empty_Subst
+      SepExpr.impures ILTac.SEP.star_SHeap SepExpr.FM.empty ILTac.SEP.liftSHeap
+      ILTac.SEP.sheapSubstU ExprUnify.empty_Subst
 
       SepExpr.pures SepExpr.impures SepExpr.other
 
-      SepTac.SEP.exists_subst ExprUnify.env_of_Subst
+      ILTac.SEP.exists_subst ExprUnify.env_of_Subst
 
-      SepTac.SEP.multimap_join SepExpr.FM.add SepExpr.FM.find SepExpr.FM.map
+      ILTac.SEP.multimap_join SepExpr.FM.add SepExpr.FM.find SepExpr.FM.map
       SepExpr.SDomain SepExpr.SDenotation
 
-      SepTac.SEP.unify_remove_all SepTac.SEP.unify_remove
+      ILTac.SEP.unify_remove_all ILTac.SEP.unify_remove
 
-      SepTac.SEP.unifyArgs
+      ILTac.SEP.unifyArgs
       ExprUnify.fold_left_2_opt ExprUnify.fold_left_3_opt
       Compare_dec.lt_eq_lt_dec nat_rec nat_rect 
 
-      ExprUnify.exprUnify SepTac.SEP.substV length ExprUnify.Subst_lookup ExprUnify.Subst_replace
+      ExprUnify.exprUnify ILTac.SEP.substV length ExprUnify.Subst_lookup ExprUnify.Subst_replace
       Expr.liftExpr Expr.exprSubstU
       Peano_dec.eq_nat_dec EquivDec.equiv_dec
       Expr.EqDec_tvar
@@ -111,15 +77,20 @@ Ltac the_cancel_simplifier :=
       Expr.well_typed 
       Expr.all2
 
-      SepTac.SEP.forallEach
-      SepTac.SEP.sheapD SepTac.SEP.sexprD
-      SepTac.SEP.starred SepTac.SEP.himp
+      ILTac.SEP.forallEach
+      ILTac.SEP.sheapD ILTac.SEP.sexprD
+      ILTac.SEP.starred ILTac.SEP.himp
       Expr.Impl Expr.Impl_
 
       Expr.is_well_typed Expr.exprD Expr.applyD
 
       orb
       Expr.Provable Expr.lookupAs
+
+      EquivDec_nat Peano_dec.eq_nat_dec
+
+      Prover.Prove Prover.Facts Prover.Learn Prover.Summarize
+      Provers.in_seq Provers.groupWith
     ].
 
 Ltac vcgen :=
@@ -127,14 +98,14 @@ Ltac vcgen :=
     unfold starB, hvarB, hpropB in *; fold hprop in *.
 
 Ltac evaluate := 
-  let plg ts pcT stT fs ps :=
-    constr:(@master_plugin_correct ts pcT stT fs ps (fun _ x => x))
+  let plg := 
+    SymIL.PluginEvaluator.composite_eval (Plugin_PtsTo.MemEval_ptsto32_correct, tt) 
   in
   let prv ts fs :=
     constr:(@Provers.transitivityProver_correct ts fs)
   in
   let unfolder ts pcT stT fs ps :=
-    constr:(@SymIL.BedrockEvaluator.DefaultEvaluator.defaultLearnHook_correct
+    constr:(@Demo.defaultLearnHook_correct
       ts fs ps)
   in
   let ssigs :=
@@ -159,3 +130,25 @@ Ltac step := match goal with
 Ltac descend := Programming.descend; reduce.
 
 Ltac sep := evaluate; descend; repeat (step; descend).
+
+(*
+Definition readS : assert := st ~> ExX, Ex v, ![ $0 =*> v * #0 ] st
+  /\ st#Rp @@ (st' ~> [| st'#Rv = v |] /\ ![ $0 =*> v * #1 ] st').
+
+Definition read := bmodule "read" {{
+  bfunction "read" [readS] {
+    Rv <- $[0];;
+    If (Rv = 0) {
+      $[0] <- 0
+    } else {
+      $[0] <- $[0]
+    } ;;
+    Rv <- $[0];;
+    Goto Rp
+  }
+}}.
+
+Theorem readOk : moduleOk read.
+  vcgen; abstract sep.
+Qed.
+*)
