src/Prover.v
@@ -1,0 +1,120 @@
+Require Import List Arith Bool.
+Require Import Expr Env.
+
+Set Implicit Arguments.
+Set Strict Implicit.
+
+(** Provers that establish [expr]-encoded facts *)
+
+Definition ProverCorrect types (fs : functions types) (summary : Type)
+    (** Some prover work only needs to be done once per set of hypotheses,
+       so we do it once and save the outcome in a summary of this type. *)
+  (valid : env types -> env types -> summary -> Prop)
+  (prover : summary -> expr types -> bool) : Prop :=
+  forall vars uvars sum,
+    valid uvars vars sum ->
+    forall goal, 
+      prover sum goal = true ->
+      ValidProp fs uvars vars goal ->
+      Provable fs uvars vars goal.
+
+Record ProverT (types : list type) : Type :=
+{ Facts : Type
+; Summarize : exprs types -> Facts
+; Learn : Facts -> exprs types -> Facts
+; Prove : Facts -> expr types -> bool
+}.
+
+Record ProverT_correct (types : list type) (P : ProverT types) (funcs : functions types) : Type :=
+{ Valid : env types -> env types -> Facts P -> Prop
+; Summarize_correct : forall uvars vars hyps, 
+  AllProvable funcs uvars vars hyps ->
+  Valid uvars vars (Summarize P hyps)
+; Learn_correct : forall uvars vars facts,
+  Valid uvars vars facts -> forall hyps,
+  AllProvable funcs uvars vars hyps ->
+  Valid uvars vars (Learn P facts hyps)
+; Prove_correct : ProverCorrect funcs Valid (Prove P)
+}.
+
+(** Generic lemmas/tactis to prove things about provers **)
+
+Lemma eq_nat_dec_correct : forall (n : nat), eq_nat_dec n n = left eq_refl.
+  induction n; provers.
+Qed.
+Hint Rewrite eq_nat_dec_correct : provers.
+
+Lemma nat_seq_dec_correct : forall (n : nat), seq_dec n n = Some eq_refl.
+  unfold seq_dec. provers.
+Qed.
+Hint Rewrite nat_seq_dec_correct : provers.
+
+
+(* Everything looks like a nail?  Try this hammer. *)
+Ltac t1 := match goal with
+             | _ => discriminate
+             | _ => progress (hnf in *; simpl in *; intuition; subst)
+             | [ x := _ : _ |- _ ] => subst x || (progress (unfold x in * ))
+             | [ H : ex _ |- _ ] => destruct H
+             | [ H : context[nth_error (updateAt ?new ?ls ?n) ?n] |- _ ] =>
+               rewrite (nth_error_updateAt new ls n) in H
+                 || rewrite nth_error_updateAt in H
+             | [ s : signature _ |- _ ] => destruct s
+             | [ H : Some _ = Some _ |- _ ] => injection H; clear H
+             | [ H : _ = Some _ |- _ ] => rewrite H in *
+             | [ H : _ === _ |- _ ] => rewrite H in *
+
+             | [ |- context[match ?E with
+                              | Const _ _ => _
+                              | Var _ => _
+                              | UVar _ => _
+                              | Func _ _ => _
+                              | Equal _ _ _ => _
+                            end] ] => destruct E
+             | [ |- context[match ?E with
+                              | None => _
+                              | Some _ => _
+                            end] ] => destruct E
+             | [ |- context[if ?E then _ else _] ] => 
+               case_eq E; intro
+             | [ |- context[match ?E with
+                              | nil => _
+                              | _ :: _ => _
+                            end] ] => destruct E
+             | [ H : _ || _ = true |- _ ] => apply orb_true_iff in H; destruct H
+             | [ _ : context[match ?E with
+                               | Const _ _ => _
+                               | Var _ => _
+                               | UVar _ => _
+                               | Func _ _ => _
+                               | Equal _ _ _ => _
+                             end] |- _ ] => destruct E
+             | [ _ : context[match ?E with
+                               | nil => _
+                               | _ :: _ => _
+                             end] |- _ ] => destruct E
+             | [ H : context[if ?E then _ else _] |- _ ] => 
+               revert H; case_eq E; do 2 intro
+             | [ _ : context[match ?E with
+                               | left _ => _
+                               | right _ => _
+                             end] |- _ ] => destruct E
+             | [ _ : context[match ?E with
+                               | tvProp => _
+                               | tvType _ => _
+                             end] |- _ ] => destruct E
+             | [ _ : context[match ?E with
+                               | None => _
+                               | Some _ => _
+                             end] |- _ ] => match E with
+                                              | context[match ?E with
+                                                          | None => _
+                                                          | Some _ => _
+                                                  end] => fail 1
+                                              | _ => destruct E
+                                            end
+
+             | [ _ : context[match ?E with (_, _) => _ end] |- _ ] => destruct E
+           end.
+
+Ltac t := repeat t1; eauto.
